Spqr.lean
@@ -6,6 +6,7 @@ import Spqr.Auxiliary.Aeneas.SpecRefl
 import Spqr.Auxiliary.Aeneas.StdNextCoreIterRangeStep
 import Spqr.Auxiliary.Aeneas.StdNextStepUsize
 import Spqr.Auxiliary.Aeneas.Vec
+import Spqr.Crypto.Hkdf
 import Spqr.Lint.Basic
 import Spqr.Lint.SpecIndent
 import Spqr.Math.Gf16.Basic
@@ -159,7 +160,7 @@ import Spqr.Specs.Encoding.Polynomial.Pt.PartialCmp
 import Spqr.Specs.Encoding.Polynomial.Pt.Serialize
 import Spqr.Specs.IncrementalMlkem768.FlipEndianness
 import Spqr.Specs.IncrementalMlkem768.Generate
-import Spqr.Specs.Kdf.Hkdf
+import Spqr.Specs.Kdf.HkdfToSlice
 import Spqr.Specs.Kdf.HkdfToVec
 import Spqr.Specs.Lib.EmptyState
 import Spqr.Specs.Lib.Error.From
